x86/RealAsmproof.v
@@ -1,0 +1,1345 @@
+Require Import Smallstep.
+Require Import Machregs.
+Require Import Asm.
+Require Import Integers.
+Require Import List.
+Require Import ZArith.
+Require Import Memtype.
+Require Import Memory.
+Require Import Archi.
+Require Import Coqlib.
+Require Import AST.
+Require Import Globalenvs.
+Require Import Events.
+Require Import Values.
+Require Import Conventions1.
+Require Import AsmFacts.
+Require Import SSAsm RealAsm.
+Require Import AsmRegs.
+Require Import Errors.
+Require Import Linking.
+
+  Section PRESERVATION.
+
+  Variable prog: Asm.program.
+  Let ge := Genv.globalenv prog.
+
+  Definition pc_at (s: state): option ((function * instruction) + external_function) :=
+    let '(State rs m) := s in
+    match rs PC with
+    | Vptr b o =>
+      match Genv.find_funct_ptr ge b with
+      | Some (Internal f) =>
+        match find_instr (Ptrofs.unsigned o) (fn_code f) with
+        | Some i => Some (inl (f,i))
+        | None => None
+        end
+      | Some (External ef) => Some (inr ef)
+      | None => None
+      end
+    | _ => None
+    end.
+
+  Inductive seq: state -> state -> Prop :=
+  | seq_intro rs1 rs2 m (REQ: forall r, r <> RA -> rs1 r = rs2 r): seq (State rs1 m) (State rs2 m).
+
+
+  Inductive match_states: state -> state -> Prop :=
+  | match_states_call_alloc
+      (rs1 rs2: regset) m1 m2
+      (REQ: forall r : preg, r <> RSP -> r <> RA -> rs1 r = rs2 r)
+      (RRSP: rs1 RSP = Val.offset_ptr (rs2 RSP) (Ptrofs.repr (size_chunk Mptr)))
+      (MEQ: Mem.storev Mptr m1 (rs2 RSP) (rs1 RA) = Some m2)
+      f ialloc
+      (PC1: pc_at (State rs1 m1) = Some (inl (f,ialloc)))
+      (ALLOC: is_alloc ialloc):
+      match_states (State rs1 m1) (State rs2 m2)
+  | match_states_call_external
+      (rs1 rs2: regset) m1 m2
+      (REQ: forall r : preg, r <> RSP -> r <> RA -> rs1 r = rs2 r)
+      (RRSP: rs1 RSP = Val.offset_ptr (rs2 RSP) (Ptrofs.repr (size_chunk Mptr)))
+      (MEQ: Mem.storev Mptr m1 (rs2 RSP) (rs1 RA) = Some m2)
+      ef
+      (PC1: pc_at (State rs1 m1) = Some (inr ef)):
+      match_states (State rs1 m1) (State rs2 m2)
+  | match_states_free_ret
+      (rs1 rs2: regset) m
+      (REQ: forall r : preg, r <> RSP -> r <> RA -> rs1 r = rs2 r)
+      (RRSP: rs1 RSP = Val.offset_ptr (rs2 RSP) ((Ptrofs.repr (size_chunk Mptr))))
+      (LOADRA: Mem.loadv Mptr m (rs2 RSP) = Some (rs1 RA))
+      f
+      (PC1: pc_at (State rs1 m) = Some (inl (f,Pret))):
+      match_states (State rs1 m) (State rs2 m)
+  | match_states_free_jmp
+      (rs1 rs2: regset) m
+      (REQ: forall r: preg, r <> RSP -> r <> RA -> rs1 r = rs2 r)
+      (RRSP: rs1 RSP = Val.offset_ptr (rs2 RSP) ((Ptrofs.repr (size_chunk Mptr))))
+      (MEQ: Mem.loadv Mptr m (rs2 RSP) = Some (rs1 RA))
+      (RANU: rs1 RA <> Vundef)
+      f ijmp
+      (PC1: pc_at (State rs1 m) = Some (inl (f,ijmp)))
+      (JMP: is_jmp ijmp):
+      match_states (State rs1 m) (State rs2 m)
+  | match_states_normal s1 s2
+                        (SEQ: seq s1 s2)
+                        (PC1: match pc_at s2 with
+                              | Some (inl (f,i)) => ~ intermediate_instruction i
+                              | Some (inr ef) => False
+                              | None => True
+                              end
+                        ):
+      match_states s1 s2
+  | match_states_stuck s1 s2
+                       (PCnone: pc_at s1 = None)
+                       (PCeq: rs_state s1 PC = rs_state s2 PC)
+                       (RAXeq: rs_state s1 RAX = rs_state s2 RAX)
+    : match_states s1 s2.
+(*loadbytesv for what ???*)
+  Lemma max_stacksize_range':
+    size_chunk Mptr <= max_stacksize <= Ptrofs.max_unsigned.
+  Proof.
+    split. unfold max_stacksize.
+    destruct Mptr; simpl; lia.
+    vm_compute. congruence.
+  Qed.
+
+ (* Hypothesis WF: wf_asm_prog ge. *)
+  (* Hypothesis main_internal: *)
+  (*   exists bmain fmain, *)
+  (*     Genv.find_symbol ge (prog_main prog) = Some bmain /\ *)
+  (*     Genv.find_funct_ptr ge bmain = Some (Internal fmain). *)
+  Lemma initial_states_match :
+    forall s1 s2,
+      SSAsm.initial_state prog s1 ->
+      initial_state prog s2 ->
+      exists s1', SSAsm.initial_state prog s1' /\ match_states s1' s2.
+  Proof.
+    Admitted.
+(*
+    simpl; intros s1 s2 IS1 IS2.
+    exists s1; split; auto. inv IS1; inv IS2.
+    inv H0; inv H2.
+    unfold ge, ge0, ge1, rs0, rs1 in *. rewrite_hyps.
+    destruct (Genv.find_funct_ptr ge bmain0) eqn:Fmain.
+    - destruct f.
+      + eapply match_states_call_alloc.
+        * intros. simpl_regs. rewrite (Pregmap.gso _ _ H0). rewrite (Pregmap.gso _ _ H1). auto.
+        * simpl_regs. simpl. f_equal.
+          rewrite Ptrofs.add_assoc. rewrite (Ptrofs.add_commut (Ptrofs.neg _)), Ptrofs.add_neg_zero. rewrite Ptrofs.add_zero. auto.
+        * simpl_regs.
+          simpl. rewrite <- Ptrofs.sub_add_opp.
+          unfold Ptrofs.sub.
+          rewrite (Ptrofs.unsigned_repr (size_chunk Mptr)).
+          rewrite (Ptrofs.unsigned_repr (Mem.stack_limit + align (size_chunk Mptr) 8)).
+          3: vm_compute; intuition congruence.
+          simpl in STORE_RETADDR. congruence.
+          generalize Mem.stack_limit_range, Mem.stack_limit_range', align_Mptr_pos. omega.
+        * simpl. simpl_regs. rewrite Fmain.
+          erewrite wf_asm_alloc_at_beginning; eauto.
+        * apply make_palloc_is_alloc.
+      + eapply match_states_call_external.
+        * intros. simpl_regs. rewrite (Pregmap.gso _ _ H0). rewrite (Pregmap.gso _ _ H1). auto.
+        * simpl_regs. simpl. f_equal.
+          rewrite Ptrofs.add_assoc. rewrite (Ptrofs.add_commut (Ptrofs.neg _)), Ptrofs.add_neg_zero. rewrite Ptrofs.add_zero. auto.
+        * simpl_regs.
+          simpl. rewrite <- Ptrofs.sub_add_opp.
+          unfold Ptrofs.sub.
+          rewrite (Ptrofs.unsigned_repr (size_chunk Mptr)).
+          rewrite (Ptrofs.unsigned_repr (Mem.stack_limit + align (size_chunk Mptr) 8)).
+          3: vm_compute; intuition congruence.
+          simpl in STORE_RETADDR. congruence.
+          generalize Mem.stack_limit_range, Mem.stack_limit_range', align_Mptr_pos. omega.
+        * simpl. simpl_regs. rewrite Fmain. eauto.
+    - eapply match_states_stuck. simpl. rewrite Fmain. auto.
+      simpl. simpl_regs. auto.
+      simpl. simpl_regs. auto.
+  Qed.
+*)
+  Lemma match_states_PC:
+    forall s1 s2,
+      match_states s1 s2 ->
+      rs_state s1 PC = rs_state s2 PC.
+  Proof.
+    intros s1 s2 MS; inv MS; try rewrite REQ by congruence; try reflexivity.
+    inv SEQ. simpl; auto. apply REQ. congruence. auto.
+  Qed.
+
+  Inductive is_builtin: instruction -> Prop :=
+  | is_builtin_intro ef args res: is_builtin (Pbuiltin ef args res).
+
+  Lemma is_builtin_dec i: is_builtin i \/ ~ is_builtin i.
+  Proof.
+    destruct i; first [right; now inversion 1|now econstructor].
+  Qed.
+
+  Lemma step_internal:
+    forall s t s'
+      (STEP: SSAsm.step ge s t s')
+      f i
+      (PCAT: pc_at s = Some (inl (f,i)))
+      (NB: ~ is_builtin i),
+      SSAsm.exec_instr ge f i (rs_state s) (m_state s) = Next (rs_state s') (m_state s') /\ t = E0.
+  Proof.
+    unfold pc_at; intros s t s'  STEP; inv STEP.
+    - rewrite H, H0, H1. inversion 1; subst. simpl. eauto.
+    - rewrite H, H0, H1. intros f0 i A; inv A. intro NIB; exfalso; apply NIB. constructor.
+    - rewrite H, H0. inversion 1.
+  Qed.
+
+  Lemma step_external_store:
+    forall s t s'
+      (STEP: SSAsm.step ge s t s')
+      ef
+      (PCAT: pc_at s = Some (inr ef)),
+    exists m2,
+      Mem.storev Mptr (m_state s) (Val.offset_ptr (rs_state s RSP) (Ptrofs.neg (Ptrofs.repr (size_chunk Mptr))))
+                 (rs_state s RA) = Some m2.
+  Proof.
+    unfold pc_at; intros s t s'  STEP; inv STEP; rewrite H, H0; try now destr.
+    inversion 1; simpl; eauto.
+    admit.
+  Admitted.
+
+  Lemma internal_step:
+    forall rs1 rs2 m1 m2 f i
+      (PCAT: pc_at (State rs1 m1) = Some (inl (f,i)))
+      (EI: SSAsm.exec_instr ge f i rs1 m1 = Next rs2 m2),
+      SSAsm.step ge (State rs1 m1) E0 (State rs2 m2).
+  Proof.
+    intros.
+    simpl in PCAT. repeat destr_in PCAT.
+    eapply SSAsm.exec_step_internal; eauto.
+  Qed.  
+
+  Lemma offset_ptr_neg_sub a b ptr:
+    (Val.offset_ptr (Val.offset_ptr ptr (Ptrofs.neg a)) (Ptrofs.sub a b)) = Val.offset_ptr ptr (Ptrofs.neg b).
+  Proof.
+    rewrite Val.offset_ptr_assoc. f_equal.
+    rewrite Ptrofs.sub_add_opp. rewrite <- Ptrofs.add_assoc.
+    rewrite (Ptrofs.add_commut (Ptrofs.neg _)). rewrite Ptrofs.add_neg_zero. apply Ptrofs.add_zero_l.
+  Qed.
+
+  Lemma offset_ptr_cancel:
+    forall ptr a,
+      (exists b o, ptr = Vptr b o) ->
+      Val.offset_ptr (Val.offset_ptr ptr a) (Ptrofs.neg a) = ptr.
+  Proof.
+    intros ptr a (b & o & EQ); subst. simpl.
+    rewrite <- Ptrofs.sub_add_opp.
+    rewrite Ptrofs.add_commut.
+    rewrite Ptrofs.sub_add_l.
+    rewrite Ptrofs.sub_idem. rewrite Ptrofs.add_zero_l. auto.
+  Qed.
+
+  Lemma eval_addrmode64_seq:
+    forall (rs rs' : regset) (REQ: forall r, r <> RA -> rs r = rs' r) a,
+      eval_addrmode64 ge a rs = eval_addrmode64 ge a rs'.
+  Proof.
+    intros.
+    unfold eval_addrmode64.
+    destr. f_equal. destr. apply REQ. congruence.
+    f_equal. destr. destr. rewrite REQ by congruence. auto.
+  Qed.
+
+  Lemma eval_addrmode32_seq:
+    forall (rs rs' : regset) (REQ: forall r, r <> RA -> rs r = rs' r) a,
+      eval_addrmode32 ge a rs = eval_addrmode32 ge a rs'.
+  Proof.
+    intros.
+    unfold eval_addrmode32.
+    destr. f_equal. destr. apply REQ. congruence.
+    f_equal. destr. destr. rewrite REQ by congruence. auto.
+  Qed.
+  
+  Lemma eval_addrmode_seq:
+    forall (rs rs' : regset) (REQ: forall r, r <> RA -> rs r = rs' r) a,
+      eval_addrmode ge a rs = eval_addrmode ge a rs'.
+  Proof.
+    unfold eval_addrmode. intros.
+    destr; eauto using eval_addrmode32_seq, eval_addrmode64_seq.
+  Qed.
+
+  Lemma eval_testcond_seq:
+    forall (rs rs' : regset) (REQ: forall r, r <> RA -> rs r = rs' r) t,
+      eval_testcond t rs = eval_testcond t rs'.
+  Proof.
+    unfold eval_testcond. intros.
+    repeat rewrite REQ by congruence. repeat destr.
+  Qed.
+  
+  Lemma exec_load_seq:
+    forall chunk m a r r' rd r0 m0,
+      seq (State r m) (State r' m) ->
+      exec_load ge chunk m a r rd = Next r0 m0 ->
+      exists r1 m1,
+        exec_load ge chunk m a r' rd = Next r1 m1.
+  Proof.
+    unfold exec_load; intros chunk m a r r' rd r0 m0 SEQ EL; repeat destr_in EL.
+    erewrite eval_addrmode_seq in Heqo. rewrite Heqo. eauto. inv SEQ; auto.
+  Qed.
+
+  Lemma exec_store_seq:
+    forall chunk m a r r' rd lrd r0 m0,
+      seq (State r m) (State r' m) ->
+      exec_store ge chunk m a r rd lrd= Next r0 m0 ->
+      rd <> RA ->
+      exists r1 m1,
+        exec_store ge chunk m a r' rd lrd = Next r1 m1.
+  Proof.
+    unfold exec_store; intros chunk m a r r' rd lrd r0 m0 SEQ EL NRA; repeat destr_in EL.
+    inv SEQ.
+    erewrite eval_addrmode_seq in Heqo. rewrite <- REQ. rewrite Heqo. eauto. auto. auto.
+  Qed.
+
+  Lemma goto_label_seq:
+    forall f l rs1 rs2 m rs' m'
+      (GL : goto_label ge f l rs1 m = Next rs' m')
+      (SEQ: rs1 PC = rs2 PC),
+    exists (rs2' : regset) (m2' : mem), goto_label ge f l rs2 m = Next rs2' m2'.
+  Proof.
+    unfold goto_label. intros. destr. rewrite <- SEQ. destr. destr. eauto.
+  Qed.
+(*
+  Lemma goto_ofs_seq:
+    forall sz ofs rs1 rs2 m rs' m'
+      (GL : goto_ofs ge sz ofs rs1 m = Next rs' m')
+      (SEQ: rs1 PC = rs2 PC),
+    exists (rs2' : regset) (m2' : mem), goto_ofs ge sz ofs rs2 m = Next rs2' m2'.
+  Proof.
+    unfold goto_ofs. intros. destr_in GL. destr_in GL. inv GL. 
+    rewrite <- SEQ, Heqo. eauto.
+  Qed.
+*)
+  Ltac force_rewrite_match H :=
+    match goal with
+      H: ?b = _ |- context [ match ?a with _ => _ end ] =>
+      cut (b = a);[ let A := fresh in intro A; rewrite <- A, H | ]
+    end.
+
+  Lemma eval_builtin_arg_eq_rs:
+    forall (rs1 rs2: regset) (REQ: forall r, r <> RA -> rs1 r = rs2 r) sp m args vargs
+      (NIN: ~ in_builtin_arg args RA),
+      eval_builtin_arg ge rs1 sp m args vargs ->
+      eval_builtin_arg ge rs2 sp m args vargs.
+  Proof.
+    induction 3; rewrite ? REQ; try econstructor; eauto.
+    intro; subst. now simpl in NIN.
+    simpl in NIN. apply IHeval_builtin_arg1. intuition.
+    simpl in NIN. apply IHeval_builtin_arg2. intuition.
+    admit. admit. (*?*)
+  Admitted.
+
+  Lemma eval_builtin_args_eq_rs:
+    forall (rs1 rs2: regset) (REQ: forall r, r <> RA -> rs1 r = rs2 r) sp m args vargs
+      (NIN: Forall (fun arg => ~ in_builtin_arg arg RA) args),
+      eval_builtin_args ge rs1 sp m args vargs ->
+      eval_builtin_args ge rs2 sp m args vargs.
+  Proof.
+    induction 3; constructor; eauto.
+    eapply eval_builtin_arg_eq_rs. 3: apply H. auto. inv NIN; auto.
+    inv NIN. apply IHlist_forall2. auto.    
+  Qed.
+
+  Lemma preg_of_not_RA:
+    forall r,
+      preg_of r <> RA.
+  Proof.
+    unfold preg_of. intros.
+    destr.
+  Qed.
+  
+  Lemma extcall_arg_eq_rs:
+    forall (rs1 rs2: regset)
+      (REQ : forall r : preg, r <> RA -> rs1 r = rs2 r)
+      m1 l arg
+      (ARGS : extcall_arg rs1 m1 l arg),
+      extcall_arg rs2 m1 l arg.
+  Proof.
+    intros rs1 rs2 REQ m1 l arg ARGS; inv ARGS.
+    - rewrite REQ.
+      econstructor. apply preg_of_not_RA.
+    - econstructor; eauto. rewrite <- REQ; eauto. congruence.
+  Qed.
+
+  Lemma extcall_arg_pair_eq_rs:
+    forall (rs1 rs2: regset)
+      (REQ : forall r : preg, r <> RA -> rs1 r = rs2 r)
+      m1 l arg
+      (ARGS : extcall_arg_pair rs1 m1 l arg),
+      extcall_arg_pair rs2 m1 l arg.
+  Proof.
+    intros; inv ARGS; econstructor; eauto using extcall_arg_eq_rs.
+  Qed.
+
+  Lemma extcall_arguments_eq_rs:
+    forall (rs1 rs2: regset)
+      (REQ : forall r : preg, r <> RA -> rs1 r = rs2 r)
+      m1 sg args
+      (ARGS : extcall_arguments rs1 m1 sg args),
+      extcall_arguments rs2 m1 sg args.
+  Proof.
+    intros rs1 rs2 REQ m1. unfold extcall_arguments.
+    induction 1; econstructor; eauto using extcall_arg_pair_eq_rs.
+  Qed.
+
+  Lemma extcall_progress:
+    forall (rs1 rs2: regset)
+      (REQ : forall r : preg, r <> RSP -> r <> RA -> rs1 r = rs2 r)
+      (RRSP : rs1 RSP = Val.offset_ptr (rs2 RSP) (Ptrofs.repr (size_chunk Mptr)))
+      m2
+      b ef
+      (FFP : Genv.find_funct_ptr ge b = Some (External ef))
+      (PC1 : rs1 PC = Vptr b Ptrofs.zero)
+      args res
+      (ARGS : extcall_arguments rs1 m2 (ef_sig ef) args)
+      ra (LOADRA: Mem.loadv Mptr m2 (rs2 RSP) = Some ra)
+      (SP_TYPE : Val.has_type (rs1 RSP) Tptr)
+      (SP_NOT_VUNDEF : rs1 RSP <> Vundef)
+      (RA_NOT_VUNDEF : ra <> Vundef)
+      m' t
+      (EXTCALL : external_call ef ge args m2 t res m'),
+    exists s2', step ge (State rs2 m2) t s2'.
+  Proof.
+    Admitted.
+(*
+    intros.
+    eexists.
+    eapply exec_step_external. rewrite <- REQ by congruence. eauto. eauto.
+    eapply extcall_arguments_eq_rs. 2: eauto. intros. apply REQ. simpl_regs.
+    setoid_rewrite Pregmap.gsspec. rewrite <- RRSP.
+    destr. apply REQ. auto. auto.
+    rewrite RRSP in SP_NOT_VUNDEF. unfold Val.offset_ptr in SP_NOT_VUNDEF. destr_in SP_NOT_VUNDEF. apply Val.Vptr_has_type.
+    eauto.
+    rewrite RRSP in SP_NOT_VUNDEF. unfold Val.offset_ptr in SP_NOT_VUNDEF. destr_in SP_NOT_VUNDEF.
+    auto. eauto. eauto.
+  Qed.
+*)
+(*  Lemma eval_ros_eq:
+    forall rs1 rs2 (REQ: forall r : preg, r <> RSP -> r <> RA -> rs1 r = rs2 r) ros (NRSP: ros <> inl RSP),
+      eval_ros ge ros rs1 = eval_ros ge ros rs2.
+  Proof.
+    unfold eval_ros. intros. destr.
+    apply REQ. congruence. congruence. 
+  Qed.
+  *)
+  Lemma real_asm_progress:
+    forall s1 s2,
+      match_states s1 s2 ->
+      safe (SSAsm.semantics prog) s1 ->
+      real_asm_inv s2 ->
+      (exists r : int, final_state s2 r) \/ (exists (t : trace) (s2' : state), step (Genv.globalenv prog) s2 t s2').
+  Proof.
+    intros s1 s2 MS SAFE SPAL.
+    destruct (SAFE _  (star_refl _ _ _)) as [(r & FS)|(t & s2' & STEP)].
+    {
+      simpl in FS. inv FS.
+      assert (pc_at (State rs m) = None).
+      - simpl. rewrite H. unfold Vnullptr. destruct ptr64; auto.
+      - inv MS; try congruence. inv SEQ.
+        left. eexists; constructor; rewrite <- REQ; eauto. congruence. congruence.
+        destruct s2. left. eexists; simpl in *; econstructor. congruence. rewrite <- RAXeq; eauto.
+    }
+    simpl in *. fold ge in STEP |- *.
+    inv MS.
+    - exploit step_internal. apply STEP. eauto. intro IB; inv IB; inv ALLOC. intros (EI & T0).
+      simpl in *. subst.
+      inv ALLOC; simpl in EI. repeat destr_in EI.
+      repeat destr_in PC1.
+      Admitted.
+(*
+      exploit wf_asm_wf_allocframe; eauto. intro A; inv A.
+      rewrite offset_ptr_neg_sub in Heqo.
+      rewrite RRSP in Heqo.
+      rewrite offset_ptr_cancel in Heqo.
+      assert (m_state s2' = m2) by congruence. subst.
+      right; do 2 eexists.
+      eapply exec_step_internal.
+      rewrite <- REQ by congruence. eauto. eauto. eauto.
+      simpl. eauto.
+      unfold Mem.storev in MEQ. destr_in MEQ. eauto.
+    - simpl in PC1. repeat destr_in PC1.
+      inv STEP; rewrite_hyps.
+      right. exists t.
+      assert (m2 = m0).
+      {
+        rewrite RRSP in SZRA.
+        rewrite offset_ptr_cancel in SZRA. congruence.
+        unfold Mem.storev in MEQ. destr_in MEQ. eauto.
+      } subst.
+      eapply extcall_progress; eauto.
+      assert (exists b o, rs2 RSP = Vptr b o).
+      {
+        unfold Mem.storev, Mem.loadv in MEQ. destruct (rs2 RSP); simpl in *; try congruence. eauto.
+      }
+      unfold Mem.storev in SZRA.
+      rewrite RRSP in SZRA. rewrite offset_ptr_cancel in SZRA; eauto.
+      destr_in SZRA.
+      simpl. erewrite Mem.load_store_same; eauto.
+      change Mptr with (chunk_of_type Tptr).
+      erewrite Val.load_result_same. auto. auto.
+    - exploit step_internal. apply STEP. eauto. intro IB; inv IB. intros (EI & T0).
+      simpl in EI. repeat destr_in EI.
+      simpl in *.
+      repeat destr_in PC1.
+      unfold Mem.loadbytesv in LOADRA. repeat destr_in LOADRA.
+      exploit Mem.loadbytes_load. apply Heqo1.
+      inv SPAL. red in RSPPTR. simpl in RSPPTR. rewrite Heqv0 in RSPPTR.
+      destruct RSPPTR as (o & EQRSP & AL);inv EQRSP; eauto.
+      intro LOAD.
+      right; do 2 eexists.
+      eapply exec_step_internal.
+      rewrite <- REQ by congruence. eauto. eauto. eauto.
+      simpl. rewrite Heqv0. simpl; rewrite LOAD. eauto.
+    - exploit step_internal. apply STEP. eauto. intro IB; inv IB; inv JMP. intros (EI & T0).
+      simpl in *.
+      repeat destr_in PC1.
+      inv JMP.
+      right; do 2 eexists.
+      eapply exec_step_internal.
+      rewrite <- REQ by congruence. eauto. eauto. eauto.
+      simpl. erewrite <- eval_ros_eq; eauto. simpl in EI; simpl; repeat destr_in EI.
+      intro; subst. eapply wf_asm_jmp_no_rsp; eauto.
+    - inversion SEQ; subst.
+      simpl in *. rewrite <- REQ in PC1 by congruence.
+      repeat destr_in PC1; subst.
+      repeat destr_in Heqo.
+      + inversion STEP; subst; rewrite_hyps.
+        destruct (is_call_dec i1).
+        {
+          destruct (SAFE _ (star_one _ _ _ _ _ STEP)) as [(r & FS)|(t & s2' & STEP2)].
+          - inv FS.
+            inv i; simpl in H6. repeat destr_in H6.
+            simpl_regs_in H1. revert H1. unfold Genv.find_funct in Heqo. destr_in Heqo. inversion 1. 
+          - assert (exists b f', Genv.find_funct_ptr ge b = Some f' /\
+                            rs' PC = Vptr b Ptrofs.zero).
+            {
+              rename H6 into EI.
+              inv i; simpl in EI; repeat destr_in EI.
+              simpl_regs. unfold Genv.find_funct in Heqo; repeat destr_in Heqo. eauto.
+            }
+            destruct H as (b & f' & FFP & PC').
+            destruct f'.
+            + inv i.
+              exploit step_internal. apply STEP2. simpl. rewrite PC'. rewrite FFP.
+              erewrite wf_asm_alloc_at_beginning; eauto. inversion 1. intros (EI & T0). subst.
+              simpl in EI. destr_in EI. inv EI.
+              right; do 2 eexists. eapply exec_step_internal. rewrite <- REQ; eauto. congruence. eauto. eauto.
+              simpl in H6. destr_in H6. inv H6. simpl. force_rewrite_match Heqo. eauto.
+              simpl_regs. rewrite <- ! REQ.
+              f_equal.
+              apply offset_ptr_neg_sub. congruence. congruence.
+            + generalize (step_external_store _ _ _ STEP2 e). simpl; rewrite PC' , FFP.
+              intro STORE; trim STORE. auto. destruct STORE as (m2' & STORE).
+              inv i.
+              simpl in H6. destr_in H6. inv H6. revert STORE. simpl_regs. intros.
+              right; do 2 eexists. eapply exec_step_internal. rewrite <- REQ; eauto. congruence. eauto. eauto.
+              simpl. rewrite <- ! REQ. rewrite STORE. eauto. congruence. congruence.
+        }
+
+        cut (exists rs2' m2', exec_instr ge f0 i1 rs2 m = Next rs2' m2').
+        intros (rs2' & m2' & EI'). right; exists E0, (State rs2' m2').
+        eapply exec_step_internal. rewrite <- REQ by congruence; eauto. eauto. eauto. eauto.
+        destruct i1; simpl in H6; simpl; eauto using exec_load_seq, exec_store_seq.
+        eapply exec_store_seq; eauto. congruence.
+        eapply exec_store_seq; eauto. congruence.
+        eapply exec_store_seq; eauto. congruence.
+        eapply exec_store_seq; eauto. congruence.
+        eapply exec_store_seq; eauto. congruence.
+        eapply exec_store_seq; eauto. congruence.
+        eapply exec_store_seq; eauto. congruence.
+        eapply exec_store_seq; eauto. congruence.
+        repeat rewrite <- REQ by congruence. repeat destr_in H6. eauto.
+        repeat rewrite <- REQ by congruence. repeat destr_in H6. eauto.
+        repeat rewrite <- REQ by congruence. repeat destr_in H6. eauto.
+        repeat rewrite <- REQ by congruence. repeat destr_in H6. eauto.
+        repeat destr; eauto.
+        eapply goto_label_seq; eauto. apply REQ; congruence.
+        erewrite <- eval_ros_eq. 2: inv SEQ; intros; apply REQ; auto. destr_in H6. eauto. intro; subst.
+        eapply wf_asm_jmp_no_rsp; eauto.
+        erewrite <- eval_testcond_seq by eauto. repeat destr_in H6; eauto. eapply goto_label_seq; eauto. apply REQ; congruence.
+        erewrite <- eval_testcond_seq by eauto. destr_in H6.
+        erewrite <- eval_testcond_seq by eauto. repeat destr_in H6; eauto. eapply goto_label_seq; eauto. apply REQ; congruence.
+        rewrite <- REQ by congruence. destr. destr. eapply goto_label_seq. eauto. simpl_regs. apply REQ; congruence.
+        exfalso; apply n; econstructor.
+        exfalso; apply PC1. constructor 2. auto.
+        eapply exec_store_seq; eauto. congruence.
+        eapply exec_store_seq; eauto. congruence.
+        eapply goto_ofs_seq; eauto. apply REQ; congruence.
+        erewrite <- eval_testcond_seq by eauto. repeat destr_in H6; eauto. eapply goto_ofs_seq; eauto. apply REQ; congruence.
+        erewrite <- eval_testcond_seq by eauto. destr_in H6.
+        erewrite <- eval_testcond_seq by eauto. repeat destr_in H6; eauto. eapply goto_ofs_seq; eauto. apply REQ; congruence.
+        rewrite <- REQ by congruence. destr. destr. eapply goto_ofs_seq. eauto. simpl_regs. apply REQ; congruence.
+        
+        eapply eval_builtin_args_eq_rs in H4. rewrite REQ in H4.
+        right; do 2 eexists. eapply exec_step_builtin. rewrite <- REQ; eauto. congruence. all: eauto. congruence.
+        eapply wf_asm_builtin_not_PC; eauto.
+
+      + inv STEP; repeat destr_in Heqo.
+    - inv STEP; simpl in *; repeat destr_in PCnone. 
+  Qed.
+*)
+  Lemma ptrofs_cancel i f s:
+    i =
+    Ptrofs.add
+      (Ptrofs.add (Ptrofs.add i s) (Ptrofs.neg f))
+      (Ptrofs.sub f s).
+  Proof.
+    rewrite ! Ptrofs.add_assoc.
+    transitivity (Ptrofs.add i Ptrofs.zero). rewrite Ptrofs.add_zero. auto.
+    f_equal.
+    rewrite Ptrofs.sub_add_opp.
+    rewrite (Ptrofs.add_commut f). rewrite <- (Ptrofs.add_assoc _ (Ptrofs.neg s)).
+    rewrite (Ptrofs.add_commut _ (Ptrofs.neg s)). rewrite (Ptrofs.add_assoc (Ptrofs.neg s)).
+    rewrite <- (Ptrofs.add_assoc _ (Ptrofs.neg s)).
+    rewrite Ptrofs.add_neg_zero. rewrite Ptrofs.add_zero_l.
+    rewrite Ptrofs.add_commut.    rewrite Ptrofs.add_neg_zero. auto.
+  Qed.
+
+  
+  Lemma offset_ptr_has_type:
+    forall ptr o,
+      Val.has_type (Val.offset_ptr ptr o) Tptr.
+  Proof.
+    intros. destruct ptr; now (simpl; auto).
+  Qed.
+
+
+  Lemma goto_label_match:
+    forall f l rs2 m2 rs2' m2' rs1,
+      (forall r: preg, r<>RA -> rs1 r = rs2 r) ->
+      goto_label ge f l rs2 m2 = Next rs2' m2' ->
+      exists rs1' m1', goto_label ge f l rs1 m2 = Next rs1' m1' /\ seq (State rs1' m1') (State rs2' m2').
+  Proof.
+    intros f l rs2 m2 rs2' m2' rs1 REQ GL2.
+    edestruct goto_label_seq as (rs1' & m1' & GL). eauto. symmetry; apply REQ. congruence. rewrite GL.
+    do 2 eexists; split; eauto.
+    unfold goto_label in GL2, GL. destr_in GL. rewrite REQ in GL by congruence.
+    repeat destr_in GL. inv GL2.
+    constructor. intros. regs_eq.
+  Qed.
+(*
+  Lemma goto_ofs_match:
+    forall sz ofs rs2 m2 rs2' m2' rs1,
+      (forall r: preg, r<>RA -> rs1 r = rs2 r) ->
+      goto_ofs ge sz ofs rs2 m2 = Next rs2' m2' ->
+      exists rs1' m1', goto_ofs ge sz ofs rs1 m2 = Next rs1' m1' /\ seq (State rs1' m1') (State rs2' m2').
+  Proof.
+    intros sz ofs rs2 m2 rs2' m2' rs1 REQ GL2.
+    edestruct goto_ofs_seq as (rs1' & m1' & GL). eauto. symmetry; apply REQ. congruence. rewrite GL.
+    do 2 eexists; split; eauto.
+    unfold goto_ofs in GL2, GL. rewrite REQ in GL by congruence.
+    repeat destr_in GL. inv GL2.
+    constructor. intros. regs_eq.
+  Qed.
+*)
+  Lemma goto_label_PC:
+    forall f l r m r0 m0
+      (GL: goto_label ge f l r m = Next r0 m0)
+      b i
+      (PCbef: r PC = Vptr b i)
+      (FFP: Genv.find_funct_ptr ge b = Some (Internal f)) ,
+      (forall f0 i2,
+          pc_at (State r0 m0) = Some (inl (f0,i2)) ->
+          ~ intermediate_instruction i2)
+      /\ (forall ef,
+            pc_at (State r0 m0) = Some (inr ef) ->
+            False ).
+  Proof.
+    intros.
+    simpl.
+    unfold goto_label in GL.
+    rewrite PCbef, FFP in GL. destr_in GL. inv GL. simpl_regs. rewrite FFP.
+    destr. split. 2: inversion 1. intros f0 i2 EQ; inv EQ.
+    Admitted.
+(*
+    assert (EQz: Ptrofs.unsigned (Ptrofs.repr z) = z).
+    {
+      replace z with (z-0) by omega.
+      admit.
+(*      eapply label_pos_repr. rewrite Z.add_0_r. eapply wf_asm_code_bounded. eauto. omega. eauto. *)
+    } rewrite EQz in *.
+    generalize (label_pos_spec l (fn_code f0) 0 z). intro LPS; trim LPS.
+    rewrite Z.add_0_r. eapply wf_asm_code_bounded; eauto. trim LPS. omega. trim LPS; auto.
+    generalize (find_instr_ofs_pos _ _ _ LPS).
+    intros POS II; inv II.
+    {
+      inv H. exploit wf_asm_alloc_only_at_beginning. eauto. apply Heqo0.
+      generalize (instr_size_positive (Plabel l)); omega.
+    }
+    {
+      exploit wf_asm_ret_jmp_comes_after_freeframe. eauto. 2: apply H.
+      rewrite EQz. eauto.
+      intros (o' & ifree & FI & IFREE & RNG).
+      generalize (find_instr_no_overlap' _ _ _ _ _ FI LPS).
+      intros [EQ|NOOV]. subst; inv IFREE.
+      rewrite EQz in *.
+      generalize (instr_size_positive ifree) (instr_size_positive (Plabel l)). omega.
+    }
+  Qed.
+*)
+Inductive is_call: instruction -> Prop :=
+| is_call_intro_r:
+    forall r sg,
+      is_call (Pcall_r r sg)
+| is_call_intro_s:
+    forall i sg,
+      is_call (Pcall_s i sg).
+Lemma is_call_dec:
+  forall i,
+    {is_call i} + {~ is_call i}.
+Proof.
+  destruct i; try now (right; intro A; inv A).
+  left; econstructor; eauto.
+  left; econstructor; eauto.
+Qed.
+
+
+  Lemma exec_instr_normal:
+    forall rs1 rs2 m1 m2 b ofs f i rs2' m2',
+      seq (State rs1 m1) (State rs2 m2) ->
+      rs2 PC = Vptr b ofs ->
+      Genv.find_funct_ptr ge b = Some (Internal f) ->
+      find_instr (Ptrofs.unsigned ofs) (fn_code f) = Some i ->
+      exec_instr ge f i rs2 m2 = Next rs2' m2' ->
+      ~ intermediate_instruction i ->
+      ~ is_call i ->
+      ~ is_free i ->
+      (exists rs1' m1',
+        SSAsm.exec_instr ge f i rs1 m1 = Next rs1' m1' /\
+        seq (State rs1' m1') (State rs2' m2')) /\
+        match pc_at (State rs2' m2') with
+        | Some (inl (_, i)) => ~ intermediate_instruction i
+        | Some (inr ef) => False
+        | None => True
+        end.
+  Proof.
+    intros rs1 rs2 m1 m2 b ofs f i rs2' m2' SEQ PC2 FFP FI EI NII NIC NIF.
+    simpl.
+    inv SEQ.
+    assert (SSAsm.exec_instr ge f i rs2 m2 = Next rs2' m2').
+    {
+      rewrite <- EI.
+      destruct i; auto.
+      contradict NIC; constructor.
+      contradict NIC; constructor.
+      contradict NII. constructor 2. auto.
+      contradict NII. constructor. constructor.
+      contradict NIF. constructor.
+    } clear EI; rename H into EI.
+    admit.
+Admitted.
+(*
+    split.
+    {
+        destruct i; simpl in *; unfold exec_load, exec_store in *;
+          erewrite ? eval_addrmode_seq by eauto;
+          repeat erewrite ?  eval_testcond_seq by eauto;
+          erewrite ? REQ by congruence;
+          repeat destr_in EI;
+          try (do 2 eexists; split; [eauto|constructor; intros; simpl; regs_eq;
+                                           try eapply eval_addrmode64_seq ; now eauto
+                                    ]; fail).
+        do 2 eexists; split; [eauto|constructor; intros; simpl; regs_eq; repeat destr; simpl; regs_eq].
+        
+        do 2 eexists; split; [eauto|constructor; intros; simpl; regs_eq; repeat destr; simpl; regs_eq].
+        eapply goto_label_match; eauto.
+        erewrite eval_ros_eq. 2: now (intros; apply REQ; auto). setoid_rewrite Heqo.
+        do 2 eexists; split; [eauto|constructor; intros; simpl; regs_eq; repeat destr; simpl; regs_eq].
+        intro; subst; eapply wf_asm_jmp_no_rsp; eauto.
+        eapply goto_label_match; eauto.
+        erewrite eval_testcond_seq by eauto. rewrite Heqo0. eapply goto_label_match; eauto.
+        erewrite eval_testcond_seq by eauto. rewrite Heqo0.
+        do 2 eexists; split; [eauto|constructor; intros; simpl; regs_eq; repeat destr; simpl; regs_eq].
+        erewrite eval_testcond_seq by eauto. rewrite Heqo0.
+        do 2 eexists; split; [eauto|constructor; intros; simpl; regs_eq; repeat destr; simpl; regs_eq].
+        eapply goto_label_match. 2: eauto. intros; regs_eq.
+        contradict NIC. constructor.
+        contradict NII. constructor 2; auto.
+        contradict NII. constructor. constructor.
+
+        eapply goto_ofs_match; eauto.
+        eapply goto_ofs_match; eauto.
+        erewrite eval_testcond_seq by eauto. rewrite Heqo0. eapply goto_ofs_match; eauto.
+        erewrite eval_testcond_seq by eauto. rewrite Heqo0.
+        do 2 eexists; split; [eauto|constructor; intros; simpl; regs_eq; repeat destr; simpl; regs_eq].
+        erewrite eval_testcond_seq by eauto. rewrite Heqo0.
+        do 2 eexists; split; [eauto|constructor; intros; simpl; regs_eq; repeat destr; simpl; regs_eq].
+        eapply goto_ofs_match. 2: eauto. intros; regs_eq.
+    }
+    destruct (Val.eq (rs2' PC) (Val.offset_ptr (rs2 PC) (Ptrofs.repr (instr_size i)))).
+    {
+      rewrite e, PC2. simpl. rewrite FFP.
+      destr. repeat destr_in Heqo. rename Heqo0 into FI'.
+      intro A.
+      inv A.
+      {
+        inv H. exploit wf_asm_alloc_only_at_beginning. eauto. apply FI'.
+        erewrite wf_asm_pc_repr; eauto.
+        generalize (Ptrofs.unsigned_range ofs) (instr_size_positive i); omega.
+      }
+      {
+        exploit wf_asm_ret_jmp_comes_after_freeframe; eauto.
+        intros (o' & ifree & FI2 & IFREE & RNG).
+        generalize (find_instr_no_overlap' _ _ _ _ _ FI FI2).
+        erewrite wf_asm_pc_repr in RNG; eauto.
+        rewrite RNG.
+        intros [EQ|NOOV]. subst. congruence.
+        generalize (instr_size_positive i) (instr_size_positive ifree). omega.
+      }
+    }
+    
+    destruct i; simpl in *; unfold exec_load, exec_store in EI; repeat destr_in EI;
+      unfold compare_ints, compare_longs, compare_floats, compare_floats32 in n;
+      repeat destr_in n;
+      simpl_regs_in n; try congruence.
+    generalize (goto_label_PC _ _ _ _ _ _ H0 _ _ PC2 FFP). simpl. intros (A & B); repeat destr; eauto.
+    contradict NII. econstructor 2. right. econstructor.
+    generalize (goto_label_PC _ _ _ _ _ _ H0 _ _ PC2 FFP). simpl. intros (A & B); repeat destr; eauto.
+    generalize (goto_label_PC _ _ _ _ _ _ H0 _ _ PC2 FFP). simpl. intros (A & B); repeat destr; eauto.
+    generalize (goto_label_PC _ _ _ _ _ _ H0 _ _ PC2 FFP). simpl. intros (A & B); repeat destr; eauto.
+    contradict NIC. constructor.
+    contradict NII. constructor 2. auto.
+    exploit find_jmp_rel_absurd; eauto. intros. contradiction.
+    exploit find_jmp_rel_absurd; eauto. intros. contradiction.
+    exploit find_jmp_rel_absurd; eauto. intros. contradiction.
+    exploit find_jmp_rel_absurd; eauto. intros. contradiction.
+
+    rewrite PC2, FFP, FI. intro A. inv A. inv H. destruct H as [H|H]; inv H.
+  Qed.
+*)
+  (*Lemma loadbytesv_storev:
+    forall m' (rs2 rs1 : regset),
+      Mem.loadbytesv Mptr m' (rs2 RSP) = Some (rs1 RA) ->
+      rs1 RA <> Vundef ->
+      bstack_perm prog (State rs2 m') ->
+      stack_top_state prog (State rs2 m') ->
+      rsp_ptr prog (State rs2 m') ->
+      Mem.storev Mptr m' (rs2 RSP) (rs1 RA) = Some m'.
+  Proof.
+    intros m' rs2 rs1 MEQ RANU BSTACK_PERM STOP RSPPTR.
+    unfold Mem.loadbytesv in MEQ; repeat destr_in MEQ. simpl.
+    edestruct (Mem.valid_access_store m' Mptr b (Ptrofs.unsigned i) (rs1 RA)) as (m2 & STORE).
+    {
+      destruct RSPPTR as (o & RSPPTR & SPAL). simpl in RSPPTR. rewrite Heqv in RSPPTR; inv RSPPTR.
+      red; repeat apply conj.
+      - red; intros. eapply BSTACK_PERM. simpl.
+        eapply Mem.loadbytes_range_perm; eauto.
+      - auto.
+      - left. eauto.
+    }
+    assert (Val.has_type (rs1 RA) Tptr).
+    {
+      revert H0; unfold Mem.encoded_ra, Mem.is_ptr; repeat destr; inversion 1.
+      unfold Vptrofs, Tptr. destr; simpl; auto. apply Val.Vptr_has_type.
+    }
+    assert (encode_val Mptr (rs1 RA) = l).
+    {
+      revert H0; unfold Mem.encoded_ra, Mem.is_ptr; repeat destr; inversion 1.
+      unfold Vptrofs, Mptr, Tptr. destr; simpl; auto. apply inj_proj_bytes in Heqo0. subst. f_equal.
+      eapply Mem.encode_decode_long; eauto. eapply Mem.loadbytes_length in Heqo. rewrite length_inj_bytes in Heqo. rewrite Heqo.
+      unfold Mptr; rewrite Heqb0; reflexivity.
+      apply inj_proj_bytes in Heqo0. subst. f_equal.
+      eapply Mem.encode_decode_int; eauto. eapply Mem.loadbytes_length in Heqo. rewrite length_inj_bytes in Heqo. rewrite Heqo.
+      unfold Mptr; rewrite Heqb0; reflexivity.
+      unfold Val.load_result in Heqv0.
+      unfold Mptr in *. unfold encode_val. destruct x86_32.Archi.ptr64 eqn:ARCHI; simpl in Heqv; repeat destr_in Heqv0.
+      eapply Mem.proj_value_inj_value; eauto. congruence.
+      eapply Mem.proj_value_inj_value; eauto. congruence.
+    }
+    subst.          
+    exploit Mem.store_same_ptr; eauto. intro; subst. auto.
+  Qed.
+*)
+(*
+  Lemma offsets_after_call_correct:
+    forall c pos o,
+      0 <= pos ->
+      In o (offsets_after_call c pos) ->
+      exists oc icall, find_instr oc c = Some icall /\  is_call icall /\ oc + instr_size icall = o - pos.
+  Proof.
+    induction c; simpl; intros; eauto.
+    easy.
+    destr_in H0.
+    - destruct H0.
+      + subst.
+        exists 0, a. rewrite zeq_true. split; auto. split; auto. omega.
+      + destruct (fun pos => IHc _ _ pos H0) as (oc & icall & INSTR & ICALL & EQ).
+        generalize (instr_size_positive a). omega.
+        exists (oc + instr_size a).
+        rewrite pred_dec_false.
+        replace (oc + instr_size a - instr_size a) with oc by omega. rewrite INSTR.
+        eexists; split; eauto. split; auto. omega.
+        generalize (instr_size_positive a) (find_instr_ofs_pos _ _ _ INSTR). omega.
+    - destruct (fun pos => IHc _ _ pos H0) as (oc & icall & INSTR & ICALL & EQ).
+      generalize (instr_size_positive a). omega.
+      exists (oc + instr_size a).
+      rewrite pred_dec_false.
+      replace (oc + instr_size a - instr_size a) with oc by omega. rewrite INSTR.
+      eexists; split; eauto. split; auto. omega.
+      generalize (instr_size_positive a) (find_instr_ofs_pos _ _ _ INSTR). omega.
+  Qed.
+*)
+  Lemma real_asm_step:
+    forall s2 t s2',
+      step (Genv.globalenv prog) s2 t s2' ->
+      forall s1 : state,
+        match_states s1 s2 ->
+        real_asm_inv s2 ->
+        safe (SSAsm.semantics prog) s1 ->
+        exists s1', SSAsm.step (Genv.globalenv prog) s1 t s1' /\ match_states s1' s2'.
+  Proof.
+    intros s2 t s2' STEP s1 MS INV SAFE. inv INV.
+    fold ge in STEP.
+    inv MS.
+    - simpl in PC1. repeat destr_in PC1.
+      rewrite REQ in Heqv by congruence.
+      inv STEP; rewrite_hyps. 2: inv ALLOC.
+      inv ALLOC. simpl in H6. inv H6.
+      eexists; split. eapply SSAsm.exec_step_internal. rewrite REQ by congruence; eauto.
+      eauto. eauto.
+      simpl. force_rewrite_match MEQ. eauto. f_equal.
+      rewrite RRSP.
+      Admitted.
+(*
+      eapply wf_asm_wf_allocframe in Heqo0; eauto. inv Heqo0.
+      unfold Mem.storev, Mem.loadv in MEQ. destruct (rs2 RSP); simpl in *; try congruence.
+      f_equal. apply ptrofs_cancel.
+      eapply match_states_normal.
+      constructor. intros. apply nextinstr_eq.
+      intros; apply set_reg_eq. intros. apply set_reg_eq. eauto.
+      auto.
+      rewrite RRSP. rewrite Val.offset_ptr_assoc. f_equal.
+      rewrite Ptrofs.sub_add_opp. rewrite Ptrofs.neg_add_distr. rewrite Ptrofs.add_commut.
+      rewrite Ptrofs.neg_involutive. auto.
+      simpl. simpl_regs. rewrite Heqv. simpl. rewrite Heqo.
+      destr. destr_in Heqo1. inv Heqo1.
+      intro A.
+      inv A.
+      {
+        inv H. exploit wf_asm_alloc_only_at_beginning. eauto. apply Heqo0. intro I0.
+        exploit wf_asm_alloc_only_at_beginning. eauto. apply Heqo2.
+        rewrite Ptrofs.add_unsigned. rewrite I0.
+        rewrite (Ptrofs.unsigned_repr (instr_size _)) by apply instr_size_repr.
+        simpl.
+        rewrite (Ptrofs.unsigned_repr (instr_size _)) by apply instr_size_repr.
+        apply not_eq_sym. apply Z.lt_neq. apply instr_size_positive.
+      }
+      {
+        exploit wf_asm_ret_jmp_comes_after_freeframe; eauto.
+        intros (o' & ifree & FI & IFREE & RNG).
+        exploit wf_asm_alloc_only_at_beginning; eauto.
+        intro FALLOC.
+        generalize (find_instr_no_overlap' _ _ _ _ _ FI Heqo0).
+        erewrite wf_asm_pc_repr in RNG; eauto.
+        rewrite RNG.
+        intros [EQ|NOOV]. subst; inv IFREE.
+        generalize (instr_size_positive (Pallocframe sz pub ora)) (instr_size_positive ifree). omega.
+      }
+    - simpl in PC1. repeat destr_in PC1.
+      rewrite REQ in Heqv by congruence.
+      inv STEP; rewrite_hyps.
+      assert (  RAC : ra_after_call ge (rs1 RA)).
+      {
+        destruct (SAFE _ (star_refl _ _ _)) as [(rr & FS)|(tt & s' & STEP)].
+        simpl in FS. inv FS. contradict H1. rewrite REQ by congruence. rewrite Heqv. inversion 1.
+        simpl in STEP.
+        rewrite <- REQ in Heqv by congruence.
+        fold ge in STEP.
+        inv STEP; rewrite_hyps; auto.
+      }
+      unfold Mem.storev in MEQ; destr_in MEQ.
+      assert (rs1 RA = ra /\ ra <> Vundef /\ Val.has_type ra Tptr).
+      {
+        simpl in *. split.
+        erewrite Mem.load_store_same in LOADRA; eauto. inv LOADRA.
+        change Mptr with (chunk_of_type Tptr).
+        symmetry.  apply Val.load_result_same.
+        revert RA_NOT_VUNDEF. unfold Val.load_result, Mptr, Tptr.
+        destruct x86_32.Archi.ptr64 eqn:PTR, (rs1 RA); simpl; try congruence. auto.
+        eapply Mem.load_type in LOADRA. 
+        change Tptr with (type_of_chunk Mptr). auto.
+      } destruct H as (RA1 & RA1U & RATYP); subst.
+      eexists; split. eapply SSAsm.exec_step_external. rewrite REQ by congruence; eauto.
+      eauto. 
+      rewrite RRSP. apply offset_ptr_has_type.
+      auto.
+      rewrite RRSP. simpl; congruence.
+      auto.
+      rewrite <- MEQ.
+      rewrite RRSP. rewrite offset_ptr_cancel. reflexivity. eauto.
+      eapply extcall_arguments_eq_rs. 2: apply H3.
+      intros. setoid_rewrite Pregmap.gsspec. rewrite <- RRSP.
+      destr. symmetry; apply REQ. auto. auto.
+      eauto. eauto. reflexivity.
+      eapply match_states_normal.
+      constructor. intros.
+      destruct (preg_eq r RSP). subst. simpl_regs.
+      rewrite set_pair_no_rsp.
+      rewrite Asmgenproof0.undef_regs_other.
+      rewrite Asmgenproof0.undef_regs_other_2.
+      auto.
+      apply rsp_not_destroyed_at_call.
+      simpl. intuition subst; congruence.
+      apply no_rsp_loc_external_result.
+      rewrite (Pregmap.gso _ _ n).
+      intros; apply set_reg_eq.
+      intros. apply set_reg_eq.
+      intros. apply set_pair_eq.
+      intros. apply undef_regs_eq.
+      intros. apply undef_regs_eq.  intros; apply REQ. congruence.
+      auto. auto. auto.
+      simpl. simpl_regs.
+      destr. destr_in Heqo0. destr_in Heqo0.
+      destruct RAC as (RAU & RAC).
+      specialize (RAC _ _ eq_refl _ Heqo1). red in RAC. destr_in RAC. destr_in Heqo0. inv Heqo0.
+      destruct (offsets_after_call_correct _ _ _ (Zle_refl _) RAC) as (oc & icall & ICALL & ISCALL & EQofs).
+      intro II; inv II.
+      {
+        inv H. exploit wf_asm_alloc_only_at_beginning. eauto. apply Heqo2.
+        generalize (find_instr_ofs_pos _ _ _ ICALL) (instr_size_positive icall). omega.
+      }
+      {
+        exploit wf_asm_ret_jmp_comes_after_freeframe; eauto.
+        intros (o' & ifree & FI & IFREE & RNG).
+        generalize (find_instr_no_overlap' _ _ _ _ _ FI ICALL).
+        rewrite Z.sub_0_r in EQofs. rewrite <- EQofs in RNG.
+        rewrite RNG.
+        rewrite <- RNG at 2.
+        intros [EQ|NOOV]. subst; inv IFREE; inv ISCALL.
+        generalize (instr_size_positive icall) (instr_size_positive ifree). omega.
+      }
+    - simpl in PC1. repeat destr_in PC1.
+      rewrite REQ in Heqv by congruence. inv STEP; rewrite_hyps.
+      assert (  RAC : ra_after_call ge (rs1 RA)).
+      {
+        destruct (SAFE _ (star_refl _ _ _)) as [(rr & FS)|(tt & s' & STEP)].
+        simpl in FS. inv FS. contradict H1. rewrite REQ by congruence. rewrite Heqv. inversion 1.
+        simpl in STEP.
+        rewrite <- REQ in Heqv by congruence.
+        fold ge in STEP.
+        inv STEP; rewrite_hyps; auto.
+        simpl in H7. destr_in H7.
+      }
+      simpl in H6. destr_in H6. inv H6.
+      assert (RAV: rs1 RA = v).
+      {
+        unfold Mem.loadbytesv in LOADRA. repeat destr_in LOADRA.
+        simpl in Heqo1.
+        edestruct Mem.load_loadbytes as (bytes & LB & DEC); eauto. rewrite Heqo2 in LB.  inv LB.
+        revert H0.
+        unfold Mem.encoded_ra, decode_val. destr. unfold Mptr, Vptrofs.
+        destruct x86_32.Archi.ptr64 eqn:?; inversion 1.
+        unfold Ptrofs.to_int64. f_equal.
+        apply Int64.eqm_samerepr.  apply Ptrofs.eqm64; auto. apply Ptrofs.eqm_sym, Ptrofs.eqm_unsigned_repr.
+        unfold Ptrofs.to_int. f_equal.
+        apply Int.eqm_samerepr.  apply Ptrofs.eqm32; auto. apply Ptrofs.eqm_sym, Ptrofs.eqm_unsigned_repr.
+        unfold Mptr. destr. simpl. unfold Mem.is_ptr. destr.
+        simpl. unfold Mem.is_ptr. destr.
+      }
+      eexists; split. eapply SSAsm.exec_step_internal. rewrite REQ by congruence; eauto. eauto. eauto.
+      simpl. rewrite pred_dec_true. eauto. eauto.      
+      apply match_states_normal.
+      + constructor. intros. rewrite ! (Pregmap.gso _ _ H). apply set_reg_eq; auto.
+        intros. 
+        setoid_rewrite Pregmap.gsspec. destr. apply REQ. auto. auto.
+      + simpl. simpl_regs.
+        destr. destr_in Heqo2. destr_in Heqo2.
+        destruct RAC as (RAU & RAC).
+        specialize (RAC _ _ RAV _ Heqo3). red in RAC. destr_in RAC. destr_in Heqo2. inv Heqo2.
+        destruct (offsets_after_call_correct _ _ _ (Zle_refl _) RAC) as (oc & icall & ICALL & ISCALL & EQofs).
+        intro II; inv II.
+        {
+          inv H. exploit wf_asm_alloc_only_at_beginning. eauto. apply Heqo4.
+          generalize (find_instr_ofs_pos _ _ _ ICALL) (instr_size_positive icall). omega.
+        }
+        {
+          exploit wf_asm_ret_jmp_comes_after_freeframe; eauto.
+          intros (o' & ifree & FI & IFREE & RNG).
+          generalize (find_instr_no_overlap' _ _ _ _ _ FI ICALL).
+          rewrite Z.sub_0_r in EQofs. rewrite <- EQofs in RNG.
+          rewrite RNG.
+          rewrite <- RNG at 2.
+          intros [EQ|NOOV]. subst; inv IFREE; inv ISCALL.
+          generalize (instr_size_positive icall) (instr_size_positive ifree). omega.
+        }
+    - simpl in PC1. repeat destr_in PC1.
+      rewrite REQ in Heqv by congruence. inv STEP; rewrite_hyps. 2: now (inv JMP).
+      inv JMP.
+      + simpl in H6. inv H6.
+        eexists; split. eapply SSAsm.exec_step_internal. rewrite REQ by congruence; eauto. eauto. eauto.
+        simpl.
+        erewrite eval_ros_eq. 2: now (intros; apply REQ; auto). fold ge. destr_in H0.
+        intro; subst; eapply wf_asm_jmp_no_rsp; eauto.
+        destr_in H0. inv H0.
+        unfold Genv.find_funct in Heqo1. repeat destr_in Heqo1.
+        destruct f.
+        * eapply match_states_call_alloc.
+          intros. apply set_reg_eq; auto.
+          simpl_regs. auto.
+          simpl_regs.
+          eapply loadbytesv_storev;eauto.
+          simpl. simpl_regs. rewrite H0.
+          erewrite wf_asm_alloc_at_beginning; eauto. constructor.
+        * eapply match_states_call_external.
+          intros. apply set_reg_eq; auto.
+          simpl_regs. auto.
+          simpl_regs.           eapply loadbytesv_storev;eauto.
+          simpl. rewrite H0. eauto.
+    - inv STEP; simpl in *; rewrite H, H0, ? H1 in PC1.
+      + destruct (is_call_dec i).
+        {
+          inv i0.
+          (* simpl in H2. destr_in H2. inv H2. *)
+          (* inv SEQ. *)
+          (* eexists; split. *)
+          (* eapply SSAsm.exec_step_internal. *)
+          (* rewrite REQ; eauto. congruence. eauto. eauto. *)
+          (* simpl. eauto. *)
+          (* edestruct wf_asm_call_target_exists as (bf & fd & SA & FFP); eauto. *)
+          (* fold ge. rewrite SA. *)
+          (* destruct fd. *)
+          (* eapply match_states_call_alloc. *)
+          (* intros. rewrite (Pregmap.gso _ _ H2). apply set_reg_eq; auto. intros; apply set_reg_eq. auto. *)
+          (* rewrite REQ; auto. congruence. *)
+          (* simpl_regs. rewrite REQ by congruence. *)
+          (* etransitivity. symmetry; apply offset_ptr_cancel. *)
+          (* unfold Mem.storev, Mem.loadv in Heqo. destruct (rs0 RSP); simpl in *; try congruence; eauto. *)
+          (* f_equal. apply Ptrofs.neg_involutive. *)
+          (* simpl_regs.  rewrite REQ by congruence. auto. *)
+          (* simpl. rewrite FFP. *)
+          (* erewrite wf_asm_alloc_at_beginning; eauto. constructor. *)
+          (* eapply match_states_call_external. *)
+          (* intros. rewrite (Pregmap.gso _ _ H2). apply set_reg_eq; auto. intros; apply set_reg_eq. auto. *)
+          (* rewrite REQ; auto. congruence. *)
+          (* simpl_regs. rewrite REQ by congruence. *)
+          (* etransitivity. symmetry; apply offset_ptr_cancel. *)
+          (* unfold Mem.storev, Mem.loadv in Heqo. destruct (rs0 RSP); simpl in *; try congruence; eauto. *)
+          (* f_equal. apply Ptrofs.neg_involutive. *)
+          (* simpl_regs.  rewrite REQ by congruence; auto. *)
+          (* simpl. rewrite FFP. eauto. *)
+          simpl in H2.
+          destruct (SAFE _ (star_refl _ _ _)) as [(rr & FS)|(t & s' & STEP)].
+          simpl in FS. inv FS. contradict H3. inv SEQ. rewrite REQ by congruence. rewrite H. inversion 1.
+          simpl in STEP. fold ge in STEP.
+          assert (t = E0).
+          {
+            inv SEQ. rewrite <- REQ in H by congruence.
+            inv STEP; rewrite_hyps; auto.
+          } subst.
+          eexists; split. eauto.
+          edestruct step_internal; eauto. inv SEQ. simpl. rewrite REQ, H, H0, H1. eauto. congruence. inversion 1.
+          simpl in H3. destr_in H3. inv H3.
+          unfold Genv.find_funct in Heqo. repeat destr_in Heqo.
+          inv SEQ. simpl in *. subst. destruct s'. simpl in *. subst.
+          destr_in H2. inv H2.
+          destruct f0.
+          eapply match_states_call_alloc.
+          intros. rewrite (Pregmap.gso _ _ H2). apply set_reg_eq; auto. intros; apply set_reg_eq. auto.
+          rewrite REQ by congruence; auto. erewrite <- eval_ros_eq. 2: intros; apply REQ; auto. eauto.
+          intro; subst; eapply wf_asm_call_no_rsp. 2: apply H1. eauto. auto.
+          simpl_regs. rewrite REQ by congruence.
+          symmetry; apply offset_ptr_cancel.
+          unfold Mem.storev, Mem.loadv in Heqo. destruct (rs0 RSP); simpl in *; try congruence; eauto.
+          rewrite <- Heqo.
+          f_equal. simpl_regs.
+          rewrite REQ by congruence; auto.
+          simpl. rewrite H5.
+          erewrite wf_asm_alloc_at_beginning; eauto. constructor.
+          eapply match_states_call_external.
+          intros. rewrite (Pregmap.gso _ _ H2). apply set_reg_eq; auto. intros; apply set_reg_eq. auto.
+          rewrite REQ by congruence; auto. erewrite <- eval_ros_eq. 2: intros; apply REQ; auto. eauto.
+          intro; subst; eapply wf_asm_call_no_rsp. 2: apply H1. eauto. auto.
+          simpl_regs. rewrite REQ by congruence.
+          symmetry; apply offset_ptr_cancel.
+          unfold Mem.storev, Mem.loadv in Heqo. destruct (rs0 RSP); simpl in *; try congruence; eauto.
+          rewrite <- Heqo.
+          rewrite REQ by congruence; auto.
+          simpl. rewrite H5. eauto.
+        }
+        destruct (is_free_dec i).
+        {
+          inv i0.
+          simpl in H2.
+          destruct (SAFE _ (star_refl _ _ _)) as [(rr & FS)|(t & s' & STEP)].
+          simpl in FS. inv FS. contradict H3. inv SEQ. rewrite REQ by congruence. rewrite H. inversion 1.
+          simpl in STEP. fold ge in STEP.
+          assert (t = E0).
+          {
+            inv SEQ. rewrite <- REQ in H by congruence.
+            inv STEP; rewrite_hyps; auto.
+          } subst.
+          eexists; split. eauto.
+          edestruct step_internal; eauto. inv SEQ. simpl. rewrite REQ, H, H0, H1 by congruence. eauto. inversion 1.
+          simpl in H3. destr_in H3. inv H3.
+          inv SEQ. simpl in *. subst. destruct s'. simpl in *. subst.
+          inv H2.
+          edestruct wf_asm_after_freeframe as (i' & FI & RJ); eauto. constructor.
+          destruct RJ as [RET|JMP].
+          - eapply match_states_free_ret.
+            intros.
+            apply nextinstr_eq.
+            rewrite (Pregmap.gso _ _ H3). simpl_regs. auto. 
+            rewrite REQ by congruence; auto. 
+            simpl_regs.
+            rewrite Val.offset_ptr_assoc. f_equal.
+            generalize (Ptrofs.repr (align (Z.max 0 sz) 8)).
+            generalize (Ptrofs.repr (size_chunk Mptr)).
+            intros. rewrite <- Ptrofs.sub_add_l.
+            rewrite Ptrofs.sub_add_opp.
+            rewrite Ptrofs.add_assoc. rewrite Ptrofs.add_neg_zero. rewrite Ptrofs.add_zero; auto.
+            simpl_regs.
+            rewrite <- Heqo. f_equal.
+            rewrite <- REQ by congruence; auto.
+            eapply wf_asm_free_spec in H1; eauto. f_equal. destruct H1 as (SZ & ORA); subst. auto.
+            simpl. simpl_regs. rewrite REQ, H by congruence. simpl. rewrite H0. rewrite FI. subst; eauto.
+          - eapply match_states_free_jmp.
+            intros.
+            apply nextinstr_eq.
+            rewrite (Pregmap.gso _ _ H3). simpl_regs. auto. 
+            rewrite REQ by congruence; auto. 
+            simpl_regs.
+            rewrite Val.offset_ptr_assoc. f_equal.
+            generalize (Ptrofs.repr (align (Z.max 0 sz) 8)).
+            generalize (Ptrofs.repr (size_chunk Mptr)).
+            intros. rewrite <- Ptrofs.sub_add_l.
+            rewrite Ptrofs.sub_add_opp.
+            rewrite Ptrofs.add_assoc. rewrite Ptrofs.add_neg_zero. rewrite Ptrofs.add_zero; auto.
+            simpl_regs.
+            rewrite <- Heqo. f_equal.
+            rewrite <- REQ by congruence; auto.
+            eapply wf_asm_free_spec in H1; eauto. f_equal. destruct H1 as (SZ & ORA); subst. auto.
+            simpl_regs.
+            unfold Mem.loadbytesv, Mem.encoded_ra, Mem.is_ptr in Heqo. repeat destr_in Heqo. inversion 1.
+            simpl. simpl_regs. rewrite REQ, H by congruence. simpl. rewrite H0. rewrite FI. subst; eauto.
+            auto.
+        }
+        destruct s1. simpl in *. fold ge.
+        edestruct exec_instr_normal as ((rs1' & m1' & EI & SEQ') & NEXT); eauto.
+        eexists; split.
+        inv SEQ. 
+        eapply SSAsm.exec_step_internal; eauto.
+        rewrite REQ by congruence; eauto.
+        apply match_states_normal. auto. auto.
+      + inv SEQ. eexists; split. eapply SSAsm.exec_step_builtin; eauto.
+        rewrite REQ by congruence; eauto.
+        eapply eval_builtin_args_eq_rs. 3: rewrite REQ by congruence; apply H2. intros; symmetry; apply REQ; auto.
+        eapply wf_asm_builtin_not_PC; eauto.
+        apply match_states_normal.
+        constructor. intros. apply nextinstr_nf_eq.
+        apply set_res_eq. apply undef_regs_eq. intros; auto.
+        simpl. simpl_regs. rewrite set_res_other.
+        rewrite Asmgenproof0.undef_regs_other_2. rewrite H; simpl. rewrite H0.
+        2: apply pc_not_destroyed_builtin.
+        2: eapply wf_asm_builtin_not_PC; eauto.
+        destr. destr_in Heqo. inv Heqo.
+        intro II; inv II.
+        {
+          inv H4. exploit wf_asm_alloc_only_at_beginning. eauto. apply Heqo0.
+          erewrite wf_asm_pc_repr; eauto.
+          apply not_eq_sym. apply Z.lt_neq.
+          generalize (Ptrofs.unsigned_range ofs) (instr_size_positive (Pbuiltin ef args res)). omega.
+        }
+        {
+          exploit wf_asm_ret_jmp_comes_after_freeframe; eauto.
+          intros (o' & ifree & FI & IFREE & RNG).
+          erewrite wf_asm_pc_repr in RNG; eauto.
+          erewrite wf_asm_pc_repr in Heqo0; eauto.
+          generalize (find_instr_no_overlap' _ _ _ _ _ FI H1).
+          rewrite RNG.
+          intros [EQ|NOOV]. subst; inv IFREE.
+          generalize (instr_size_positive (Pbuiltin ef args res)) (instr_size_positive ifree). omega.
+        }
+      + easy.
+    - destruct s1. simpl in *. rewrite PCeq in PCnone.
+      inv STEP; simpl in *; repeat destr_in PCnone.
+  Qed.
+*)
+  Hypothesis prog_no_rsp: asm_prog_unchange_rsp ge.
+  
+  Theorem real_asm_correct:
+    backward_simulation (SSAsm.semantics prog) (RealAsm.semantics prog).
+  Proof.
+    eapply backward_simulation_plus
+      with (match_states := fun s1 s2 => match_states s1 s2 /\ real_asm_inv s2).
+    - reflexivity.
+    - simpl; intros s1 IS1. inv IS1. inv H0. admit.
+(*
+      edestruct (Mem.valid_access_store m3 Mptr bstack0 (Mem.stack_limit + align (size_chunk Mptr) 8 - size_chunk Mptr) Vnullptr).
+      split;[|split].
+      red; intros. repeat rewrite_perms. rewrite peq_true. split.
+      cut (size_chunk Mptr <=  Mem.stack_limit). generalize align_Mptr_pos. omega. apply stack_limit_range'.
+      constructor.
+      apply Z.divide_sub_r.
+      apply Z.divide_add_r.
+      apply align_Mptr_stack_limit.
+      apply align_Mptr_align8.
+      apply align_size_chunk_divides.
+      intros.
+      red. rewrite_stack_blocks. intro. left. unfold is_stack_top. simpl. auto.
+      eexists; econstructor. eauto. econstructor; eauto.
+      simpl.
+      rewrite Ptrofs.unsigned_repr. eauto. 
+      generalize stack_limit_range'. generalize Mem.stack_limit_range'. generalize (size_chunk_pos Mptr).
+      generalize (align_le (size_chunk Mptr) 8).
+      omega. *)
+    - simpl; intros s1 s2 IS1 IS2.
+      edestruct initial_states_match as (s1' & IS1' & MS); eauto.
+      eexists; split; eauto. split; auto. admit. (*eapply real_initial_inv; eauto.*)
+    - simpl; intros s1 s2 r (MS & INV) FS; inv FS.
+      assert (pc_at s1 = None).
+      {
+        generalize (match_states_PC _ _ MS). intros PCeq.
+        unfold pc_at. destr.  simpl in *. rewrite PCeq.
+        rewrite H. unfold Vnullptr. destruct ptr64; simpl; auto.
+      }
+      inv MS; try congruence.
+      inv SEQ. simpl in *.
+      constructor. rewrite REQ by congruence. auto. rewrite REQ; auto. congruence.
+      destruct s1; simpl in *. constructor. congruence. congruence. 
+    - simpl. intros s1 s2 (MS & INV) SAFE; eapply real_asm_progress; eauto.
+    - simpl. intros s2 t s2' STEP s1 (MS & INV) SAFE.
+      edestruct real_asm_step as (s1' & STEP' & MS'); eauto.
+      exists s1'; split; eauto. apply plus_one; auto. split; auto.
+      admit. (*
+      eapply real_asm_inv_inv; eauto. *)
+  Admitted.
+
+  End PRESERVATION.
+
+Definition transf_program (p: Asm.program) : Asm.program := p.
+
+Definition match_prog (p :Asm.program) (tp:Asm.program):= p = tp.
+
+Lemma transf_program_match:
+  forall p, match_prog p (transf_program p).
+Proof.
+  intros. reflexivity.
+Qed.
+
+  Lemma match_prog_inv: forall t tp,
+    match_prog t tp -> t = tp.
+  Proof.
+    intros t tp MT. red in MT. auto.
+  Qed.
+
+  Section PRESERVATION2.
+
+  Variable prog: Asm.program.
+  Variable tprog: Asm.program.
+  Hypothesis TRANSF: match_prog prog tprog.
+  Let ge := Genv.globalenv prog.
+
+(*  Hypothesis WF: wf_asm_prog ge. *)
+  Hypothesis prog_no_rsp: asm_prog_unchange_rsp ge.
+
+  Theorem real_asm_correct':
+    backward_simulation (SSAsm.semantics prog) (RealAsm.semantics tprog).
+  Proof.
+    red in TRANSF.
+    unfold transf_program in TRANSF.
+    exploit match_prog_inv; eauto. intros EQ. subst.
+    apply real_asm_correct; auto.
+  Qed.
+
+  End PRESERVATION2.
+
