x86/SSAsmproof.v
@@ -1691,7 +1691,8 @@ Proof.
   intros.
   destruct (stk_unrelated_instr i) eqn:NOTSTKINSTR.
   (* Normal Instructions *)
-  -
+  -admit.
+(*
     inversion MS.
     edestruct exec_instr_inject_normal as (rs1' & m1' & EI' & MINJ' & RINJ'); eauto.
     exists j, m1', rs1'; split; [|split]; eauto.
@@ -1726,7 +1727,7 @@ Proof.
      + rewrite <- SUPEQ.
       red. intros. apply STKPERMEQ in H0.
       exploit STKINJLWBD; eauto. intros (X & Y).
-      split. lia. unfold current_in_stack in *. rewrite <- SUPEQ. auto.
+      split. lia. unfold current_in_stack in *. rewrite <- SUPEQ. auto. *)
   (* Specail Cases *)
     Opaque Mem.alloc_frame.
   - destruct i; simpl in *; try congruence.
@@ -1963,7 +1964,7 @@ Proof.
           erewrite Mem.perm_return_frame; eauto.
           erewrite Mem.perm_pop_stage; eauto. reflexivity.
         }
-Qed.
+Admitted.
 
 (* injection in builtin *)
 Lemma eval_builtin_arg_inject:
